minor corrections

ObcToClight/Correctness.v
@@ -346,17 +346,6 @@ Proof.
   contradict Pref; apply glob_id_not_prefixed.
 Qed.
 
-Lemma main_not_glob:
-  forall (xs: list (ident * type)),
-    ~ In main_id (map (fun xt => glob_id (fst xt)) xs).
-Proof.
-  induction xs as [|(x, t)]; simpl; auto.
-  intros [Hin|Hin].
-  - unfold glob_id, main_id in Hin.
-    apply pos_of_str_injective in Hin; inv Hin.
-  - contradiction.
-Qed.
-
 Lemma NoDupMembers_glob:
   forall (ys xs: list (ident * type)),
     NoDupMembers (xs ++ ys) ->
@@ -567,9 +556,12 @@ Section PRESERVATION.
                     map fst (concat funs) ++
                     [main_id])) as Notin_self.
     { pose proof (m_notreserved self m (in_eq self _)) as Res; unfold meth_vars in Res.
-      repeat rewrite in_app_iff, in_map_iff; rewrite In_singleton;
-        intros [((x, t) & E & Hin)|[((x, t) & E & Hin)|[((x, t) & E & Hin)|Hin]]];
-        try simpl in E.
+      repeat rewrite in_app_iff, in_map_iff; simpl;  
+        intros [((x, t) & E & Hin) 
+               |[((x, t) & E & Hin) 
+                |[((x, t) & E & Hin) 
+                 |[Hin|Hin]]]]; 
+        try simpl in E; try (apply pos_of_str_injective in Hin; now inv Hin); try contradiction. 
       - apply glob_id_injective in E; subst x.
         apply In_InMembers in Hin.
         apply Res; now repeat (rewrite InMembers_app; right).
@@ -580,31 +572,35 @@ Section PRESERVATION.
         apply in_map with (f:=fst) in Hin.
         subst funs. apply prefixed_funs, prefixed_fun_prefixed in Hin.
         contradict Hin; apply glob_id_not_prefixed. 
-      - unfold glob_id, main_id in Hin.
-        apply pos_of_str_injective in Hin.
-        inv Hin.
     }
     assert (NoDup (map (fun xt => glob_id (fst xt)) (m_out m) ++
                        map (fun xt => glob_id (fst xt)) (m_in m) ++
                        map fst (concat funs) ++
                        [main_id])) as Nodup.
     { repeat apply NoDup_app'; repeat apply Forall_not_In_app;
-        repeat apply Forall_not_In_singleton.
+        repeat apply Forall_not_In_singleton;
+        ((repeat constructor; auto) 
+         || (intros [E|]; try contradiction;  
+            apply pos_of_str_injective in E; inv E) 
+         || (intro Hin; subst funs; apply prefixed_funs in Hin; 
+            inversion Hin as [? ? E]; 
+            unfold prefix_fun, fun_id in E; 
+            apply pos_of_str_injective in E; rewrite pos_to_str_equiv in E; 
+            inv E) 
+         || (match goal with 
+              |- ~ In _ (map (fun xt => glob_id (fst xt)) ?xs) => 
+              clear Notin_self; induction xs as [|(x, t)]; simpl; auto; 
+              intros [Hin|Hin]; try contradiction; 
+              apply pos_of_str_injective in Hin; inv Hin 
+            end) 
+         || idtac). 
       - apply NoDup_glob_id, m_nodupout.
       - apply NoDup_glob_id, m_nodupin.
       - rewrite Funs.
         now apply NoDup_funs.
-      - repeat constructor; auto.
-      - intro Hin; subst funs; apply prefixed_funs in Hin.
-        inversion Hin as [? ? E].
-        unfold prefix, main_id in E.
-        unfold prefix_fun, fun_id in E.
-        apply pos_of_str_injective in E; rewrite pos_to_str_equiv in E.
-        inversion E.
       - apply glob_not_in_prefixed, all_In_Forall; intros ** Hin.
         apply prefixed_fun_prefixed; subst funs.
         now apply prefixed_funs in Hin.
-      - apply main_not_glob. 
       - apply NoDupMembers_glob.
         pose proof (m_nodupvars m) as Nodup.
         rewrite NoDupMembers_app_assoc, <-app_assoc in Nodup.
@@ -612,7 +608,6 @@ Section PRESERVATION.
       - apply glob_not_in_prefixed, all_In_Forall; intros ** Hin.
         apply prefixed_fun_prefixed; subst funs.
         now apply prefixed_funs in Hin.
-      - apply main_not_glob.
     }
     repeat constructor; auto.
   Qed.
@@ -3852,14 +3847,7 @@ Section PRESERVATION.
                                  | _ :: _ => [(prefix out step, type_of_inst (prefix_fun main_node step))]
                                  end
               /\ main.(fn_temps) = map translate_param (m_in m_step)
-              /\ main.(fn_body) =
-                 return_zero
-                   (Ssequence (reset_call main_node)
-                              (Sloop (Ssequence (load_in (m_in m_step))
-                                                (Ssequence
-                                                   (step_call main_node (map make_in_arg (m_in m_step)) (m_out m_step))
-                                                   (write_out main_node (m_out m_step))))
-                                     Sskip))
+              /\ main.(fn_body) = main_body main_node m_step
               /\ match m_out m_step with
                 | [] => True
                 | _ =>
@@ -4115,16 +4103,7 @@ Section PRESERVATION.
                                                 | _ :: _ => [(prefix out step, type_of_inst (prefix_fun main_node step))]
                                                 end
                            /\ main_f.(fn_temps) = map translate_param (m_in m_step)
-                           /\ main_f.(fn_body) =
-                             return_zero
-                               (Ssequence (reset_call main_node)
-                                          (Sloop
-                                             (Ssequence (load_in (m_in m_step))
-                                                        (Ssequence
-                                                           (step_call main_node
-                                                                      (map make_in_arg (m_in m_step))
-                                                                      (m_out m_step))
-                                                           (write_out main_node (m_out m_step)))) Sskip)).
+                           /\ main_f.(fn_body) = main_body main_node m_step.
 
     Hypothesis Getstep_co: match m_step.(m_out) with
                            | [] => True
@@ -4628,22 +4607,15 @@ Section PRESERVATION.
       (** Correctness of the main loop                                 *)
       (*****************************************************************)
 
-      Definition body :=
-        Ssequence
-          (load_in (m_in m_step))
-          (Ssequence
-             (step_call main_node
-                        (map make_in_arg (m_in m_step)) (m_out m_step))
-             (write_out main_node (m_out m_step))).
-
       Lemma exec_body:
         forall n meN le,
           dostep' n meN ->
           exists leSn meSn,
             exec_stmt (globalenv tprog) (function_entry2 (globalenv tprog)) e1 le meN
-                      body (load_events (map sem_const (ins n)) (m_in m_step)
-                                        ++ E0
-                                        ++ store_events (map sem_const (outs n)) (m_out m_step))
+                      (main_loop_body main_node m_step)
+                      (load_events (map sem_const (ins n)) (m_in m_step)
+                       ++ E0
+                       ++ store_events (map sem_const (outs n)) (m_out m_step))
                       leSn meSn Out_normal
             /\ dostep' (S n) meSn.
       Proof.
@@ -4785,10 +4757,6 @@ Section PRESERVATION.
         eapply exec_write; eauto.
       Qed.    
 
-      Definition loop := 
-        (* XXX: factor it out in [Generation.v] *)
-        Sloop body Sskip.
-
       Definition transl_trace (n: nat): traceinf' :=
         trace_step m_step ins outs Step_in_spec Step_out_spec Hwt_ins Hwt_outs n.
 
@@ -4797,7 +4765,8 @@ Section PRESERVATION.
           wt_mem meInit prog_main c_main ->
           dostep' n me ->
           execinf_stmt (globalenv tprog) (function_entry2 (globalenv tprog)) e1 le me
-                       loop (traceinf_of_traceinf' (transl_trace n)).
+                       (main_loop main_node m_step)
+                       (traceinf_of_traceinf' (transl_trace n)).
       Proof.
         cofix COINDHYP.
         intros ** Hdostep.
@@ -4887,7 +4856,7 @@ Section PRESERVATION.
         forall n m le,
           dostep' n m ->
           Smallstep.forever_reactive (step_fe function_entry2) (globalenv tprog)
-                                     (Clight.State main_f loop after_loop e1 le m)
+                                     (Clight.State main_f (main_loop main_node m_step) after_loop e1 le m)
                                      (traceinf_of_traceinf' (transl_trace n)).
       Proof.
         unfold transl_trace, trace_step.
@@ -4896,7 +4865,7 @@ Section PRESERVATION.
         edestruct exec_body with (1:=Hdostep') as (? & ? & Exec_body & ?).
         eapply exec_stmt_steps in Exec_body.
         destruct Exec_body as (? & Star_body & Out_body).
-        unfold body in Star_body.      
+        unfold main_loop_body in Star_body.      
         rewrite unfold_mk_trace.
 
         econstructor; simpl.
@@ -5005,9 +4974,8 @@ Section PRESERVATION.
       as (? & ? & ? & ? & ? & ? & ? & ? & ? & ? & ? & ?); eauto.
     intros.
     case_eq (m_out m_step); intros ** Out;
-      rewrite Out in Hmout, Hvars, Hbody.
-    - (* destruct Hmout as (? & ? & ?). *)
-      eapply reacts; try rewrite Out; eauto.
+      rewrite Out in Hmout, Hvars. 
+    - eapply reacts; try rewrite Out; eauto. 
       + repeat split; auto.
       + rewrite Hvars; econstructor.
       + erewrite <-sepemp_left, <-sepemp_right; eauto.
